EC/passCertRPG_jazz.ec
@@ -4,29 +4,36 @@ from Jasmin require import JModel.
 require import Array76.
 require import WArray76.
 
-op [full uniform] RDRAND: W64.t distr.   
+op [full uniform] RDRAND: W64.t distr.
 
 module M = {
   proc rng (range:W64.t) : W64.t = {
     
-    var tmp2:W64.t;
-    var max_value:W64.t;
     var tmp1:W64.t;
-    var rand_number:W64.t;
+    var tmp2:W64.t;
+    var tmp_range:W64.t;
+    var max_value:W64.t;
     
-    max_value <- (W64.of_int 18446744073709551615);
-    tmp1 <- range;
-    max_value <- (max_value \udiv tmp1);
-    max_value <- (max_value * tmp1);
-    max_value <- (max_value - (W64.of_int 1));
-    rand_number <$ RDRAND ;
-    
-    while ((max_value \ult rand_number)) {
-      rand_number <$ RDRAND ;
+    tmp1 <- (W64.of_int 18446744073709551615);
+    tmp2 <- (W64.of_int 18446744073709551615);
+    tmp_range <- range;
+    tmp1 <- (tmp1 \umod tmp_range);
+    tmp_range <- (tmp_range - (W64.of_int 1));
+    if ((tmp1 = tmp_range)) {
+      max_value <- tmp2;
+    } else {
+      max_value <- (tmp2 - tmp1);
+      max_value <- (max_value - (W64.of_int 1));
     }
-    tmp2 <- rand_number;
-    tmp2 <- (tmp2 \umod tmp1);
-    return (tmp2);
+    tmp2 <$ RDRAND ;
+    
+    while ((max_value \ult tmp2)) {
+      tmp2 <$ RDRAND ;
+    }
+    tmp1 <- tmp2;
+    tmp_range <- (tmp_range + (W64.of_int 1));
+    tmp1 <- (tmp1 \umod tmp_range);
+    return (tmp1);
   }
   
   proc random_char_generator (range:W64.t, set:W8.t Array76.t) : W8.t = {
@@ -168,304 +175,333 @@ module M = {
     special_max <-
     (loadW64 Glob.mem (W64.to_uint (policy_addr + (W64.of_int 64))));
     tmp64_1 <- length;
-    if ((tmp64_1 \sle (W64.of_int 200))) {
-      if (((W64.of_int 0) \sle tmp64_1)) {
+    if ((tmp64_1 \ule (W64.of_int 200))) {
+      if (((W64.of_int 0) \ult tmp64_1)) {
         tmp64_1 <- lowercase_min;
-        if (((W64.of_int 0) \sle tmp64_1)) {
+        if (((W64.of_int 0) \ule tmp64_1)) {
           tmp64_1 <- uppercase_min;
-          if (((W64.of_int 0) \sle tmp64_1)) {
+          if (((W64.of_int 0) \ule tmp64_1)) {
             tmp64_1 <- numbers_min;
-            if (((W64.of_int 0) \sle tmp64_1)) {
+            if (((W64.of_int 0) \ule tmp64_1)) {
               tmp64_1 <- special_min;
-              if (((W64.of_int 0) \sle tmp64_1)) {
+              if (((W64.of_int 0) \ule tmp64_1)) {
                 tmp64_1 <- lowercase_max;
-                tmp64_2 <- lowercase_min;
-                if ((tmp64_2 \ule tmp64_1)) {
+                if ((tmp64_1 \ule (W64.of_int 200))) {
                   tmp64_1 <- uppercase_max;
-                  tmp64_2 <- uppercase_min;
-                  if ((tmp64_2 \ule tmp64_1)) {
+                  if ((tmp64_1 \ule (W64.of_int 200))) {
                     tmp64_1 <- numbers_max;
-                    tmp64_2 <- numbers_min;
-                    if ((tmp64_2 \ule tmp64_1)) {
+                    if ((tmp64_1 \ule (W64.of_int 200))) {
                       tmp64_1 <- special_max;
-                      tmp64_2 <- special_min;
-                      if ((tmp64_2 \ule tmp64_1)) {
-                        tmp64_1 <- lowercase_min;
-                        tmp64_2 <- uppercase_min;
-                        tmp64_1 <- (tmp64_1 + tmp64_2);
-                        tmp64_2 <- numbers_min;
-                        tmp64_1 <- (tmp64_1 + tmp64_2);
-                        tmp64_2 <- special_min;
-                        tmp64_1 <- (tmp64_1 + tmp64_2);
-                        if ((tmp64_1 \ule length)) {
-                          tmp64_1 <- lowercase_max;
-                          tmp64_2 <- uppercase_max;
-                          tmp64_1 <- (tmp64_1 + tmp64_2);
-                          tmp64_2 <- numbers_max;
-                          tmp64_1 <- (tmp64_1 + tmp64_2);
-                          tmp64_2 <- special_max;
-                          tmp64_1 <- (tmp64_1 + tmp64_2);
-                          if ((length \ule tmp64_1)) {
-                            lowercase_set.[0] <- (W8.of_int 97);
-                            lowercase_set.[1] <- (W8.of_int 98);
-                            lowercase_set.[2] <- (W8.of_int 99);
-                            lowercase_set.[3] <- (W8.of_int 100);
-                            lowercase_set.[4] <- (W8.of_int 101);
-                            lowercase_set.[5] <- (W8.of_int 102);
-                            lowercase_set.[6] <- (W8.of_int 103);
-                            lowercase_set.[7] <- (W8.of_int 104);
-                            lowercase_set.[8] <- (W8.of_int 105);
-                            lowercase_set.[9] <- (W8.of_int 106);
-                            lowercase_set.[10] <- (W8.of_int 107);
-                            lowercase_set.[11] <- (W8.of_int 108);
-                            lowercase_set.[12] <- (W8.of_int 109);
-                            lowercase_set.[13] <- (W8.of_int 110);
-                            lowercase_set.[14] <- (W8.of_int 111);
-                            lowercase_set.[15] <- (W8.of_int 112);
-                            lowercase_set.[16] <- (W8.of_int 113);
-                            lowercase_set.[17] <- (W8.of_int 114);
-                            lowercase_set.[18] <- (W8.of_int 115);
-                            lowercase_set.[19] <- (W8.of_int 116);
-                            lowercase_set.[20] <- (W8.of_int 117);
-                            lowercase_set.[21] <- (W8.of_int 118);
-                            lowercase_set.[22] <- (W8.of_int 119);
-                            lowercase_set.[23] <- (W8.of_int 120);
-                            lowercase_set.[24] <- (W8.of_int 121);
-                            lowercase_set.[25] <- (W8.of_int 122);
-                            i <- (W64.of_int 26);
-                            
-                            while ((i \ult (W64.of_int 76))) {
-                              lowercase_set.[(W64.to_uint i)] <-
-                              (W8.of_int 0);
-                              i <- (i + (W64.of_int 1));
-                            }
-                            uppercase_set.[0] <- (W8.of_int 65);
-                            uppercase_set.[1] <- (W8.of_int 66);
-                            uppercase_set.[2] <- (W8.of_int 67);
-                            uppercase_set.[3] <- (W8.of_int 68);
-                            uppercase_set.[4] <- (W8.of_int 69);
-                            uppercase_set.[5] <- (W8.of_int 70);
-                            uppercase_set.[6] <- (W8.of_int 71);
-                            uppercase_set.[7] <- (W8.of_int 72);
-                            uppercase_set.[8] <- (W8.of_int 73);
-                            uppercase_set.[9] <- (W8.of_int 74);
-                            uppercase_set.[10] <- (W8.of_int 75);
-                            uppercase_set.[11] <- (W8.of_int 76);
-                            uppercase_set.[12] <- (W8.of_int 77);
-                            uppercase_set.[13] <- (W8.of_int 78);
-                            uppercase_set.[14] <- (W8.of_int 79);
-                            uppercase_set.[15] <- (W8.of_int 80);
-                            uppercase_set.[16] <- (W8.of_int 81);
-                            uppercase_set.[17] <- (W8.of_int 82);
-                            uppercase_set.[18] <- (W8.of_int 83);
-                            uppercase_set.[19] <- (W8.of_int 84);
-                            uppercase_set.[20] <- (W8.of_int 85);
-                            uppercase_set.[21] <- (W8.of_int 86);
-                            uppercase_set.[22] <- (W8.of_int 87);
-                            uppercase_set.[23] <- (W8.of_int 88);
-                            uppercase_set.[24] <- (W8.of_int 89);
-                            uppercase_set.[25] <- (W8.of_int 90);
-                            i <- (W64.of_int 26);
-                            
-                            while ((i \ult (W64.of_int 76))) {
-                              uppercase_set.[(W64.to_uint i)] <-
-                              (W8.of_int 0);
-                              i <- (i + (W64.of_int 1));
-                            }
-                            numbers_set.[0] <- (W8.of_int 48);
-                            numbers_set.[1] <- (W8.of_int 49);
-                            numbers_set.[2] <- (W8.of_int 50);
-                            numbers_set.[3] <- (W8.of_int 51);
-                            numbers_set.[4] <- (W8.of_int 52);
-                            numbers_set.[5] <- (W8.of_int 53);
-                            numbers_set.[6] <- (W8.of_int 54);
-                            numbers_set.[7] <- (W8.of_int 55);
-                            numbers_set.[8] <- (W8.of_int 56);
-                            numbers_set.[9] <- (W8.of_int 57);
-                            i <- (W64.of_int 10);
-                            
-                            while ((i \ult (W64.of_int 76))) {
-                              numbers_set.[(W64.to_uint i)] <- (W8.of_int 0);
-                              i <- (i + (W64.of_int 1));
-                            }
-                            special_set.[0] <- (W8.of_int 33);
-                            special_set.[1] <- (W8.of_int 63);
-                            special_set.[2] <- (W8.of_int 35);
-                            special_set.[3] <- (W8.of_int 36);
-                            special_set.[4] <- (W8.of_int 37);
-                            special_set.[5] <- (W8.of_int 38);
-                            special_set.[6] <- (W8.of_int 43);
-                            special_set.[7] <- (W8.of_int 45);
-                            special_set.[8] <- (W8.of_int 42);
-                            special_set.[9] <- (W8.of_int 95);
-                            special_set.[10] <- (W8.of_int 64);
-                            special_set.[11] <- (W8.of_int 58);
-                            special_set.[12] <- (W8.of_int 59);
-                            special_set.[13] <- (W8.of_int 61);
-                            i <- (W64.of_int 14);
-                            
-                            while ((i \ult (W64.of_int 76))) {
-                              special_set.[(W64.to_uint i)] <- (W8.of_int 0);
-                              i <- (i + (W64.of_int 1));
-                            }
-                            i <- (W64.of_int 0);
-                            
-                            while ((i \ult (W64.of_int 76))) {
-                              union_set.[(W64.to_uint i)] <- (W8.of_int 0);
-                              i <- (i + (W64.of_int 1));
-                            }
-                            i_filled <- (W64.of_int 0);
-                            if (((W64.of_int 0) \ult lowercase_max)) {
-                              i <- (W64.of_int 0);
-                              
-                              while ((i \ult lowercase_min)) {
-                                lowercase_max <-
-                                (lowercase_max - (W64.of_int 1));
-                                tmp8 <@ random_char_generator ((W64.of_int 26),
-                                lowercase_set);
-                                Glob.mem <-
-                                storeW8 Glob.mem (W64.to_uint (output_addr + i_filled)) tmp8;
-                                i <- (i + (W64.of_int 1));
-                                i_filled <- (i_filled + (W64.of_int 1));
-                              }
-                            } else {
-                              
-                            }
-                            if (((W64.of_int 0) \ult uppercase_max)) {
-                              i <- (W64.of_int 0);
-                              
-                              while ((i \ult uppercase_min)) {
-                                uppercase_max <-
-                                (uppercase_max - (W64.of_int 1));
-                                tmp8 <@ random_char_generator ((W64.of_int 26),
-                                uppercase_set);
-                                Glob.mem <-
-                                storeW8 Glob.mem (W64.to_uint (output_addr + i_filled)) tmp8;
-                                i <- (i + (W64.of_int 1));
-                                i_filled <- (i_filled + (W64.of_int 1));
-                              }
-                            } else {
-                              
-                            }
-                            if (((W64.of_int 0) \ult numbers_max)) {
-                              i <- (W64.of_int 0);
-                              
-                              while ((i \ult numbers_min)) {
-                                numbers_max <-
-                                (numbers_max - (W64.of_int 1));
-                                tmp8 <@ random_char_generator ((W64.of_int 10),
-                                numbers_set);
-                                Glob.mem <-
-                                storeW8 Glob.mem (W64.to_uint (output_addr + i_filled)) tmp8;
-                                i <- (i + (W64.of_int 1));
-                                i_filled <- (i_filled + (W64.of_int 1));
-                              }
-                            } else {
-                              
-                            }
-                            if (((W64.of_int 0) \ult special_max)) {
-                              i <- (W64.of_int 0);
-                              
-                              while ((i \ult special_min)) {
-                                special_max <-
-                                (special_max - (W64.of_int 1));
-                                tmp8 <@ random_char_generator ((W64.of_int 14),
-                                special_set);
-                                Glob.mem <-
-                                storeW8 Glob.mem (W64.to_uint (output_addr + i_filled)) tmp8;
-                                i <- (i + (W64.of_int 1));
-                                i_filled <- (i_filled + (W64.of_int 1));
-                              }
-                            } else {
-                              
-                            }
-                            (tmp64_1,
-                            union_set) <@ define_union_set (lowercase_max,
-                            uppercase_max, numbers_max, special_max,
-                            lowercase_set, uppercase_set, numbers_set,
-                            special_set, union_set);
-                            tmp64_2 <- length;
-                            
-                            while ((i_filled \ult tmp64_2)) {
-                              tmp8 <@ random_char_generator (tmp64_1,
-                              union_set);
-                              if (((W8.of_int 97) \ule tmp8)) {
-                                if ((tmp8 \ule (W8.of_int 122))) {
-                                  lowercase_max <-
-                                  (lowercase_max - (W64.of_int 1));
-                                  if ((lowercase_max = (W64.of_int 0))) {
+                      if ((tmp64_1 \ule (W64.of_int 200))) {
+                        tmp64_1 <- lowercase_max;
+                        tmp64_2 <- lowercase_min;
+                        if ((tmp64_2 \ule tmp64_1)) {
+                          tmp64_1 <- uppercase_max;
+                          tmp64_2 <- uppercase_min;
+                          if ((tmp64_2 \ule tmp64_1)) {
+                            tmp64_1 <- numbers_max;
+                            tmp64_2 <- numbers_min;
+                            if ((tmp64_2 \ule tmp64_1)) {
+                              tmp64_1 <- special_max;
+                              tmp64_2 <- special_min;
+                              if ((tmp64_2 \ule tmp64_1)) {
+                                tmp64_1 <- lowercase_min;
+                                tmp64_2 <- uppercase_min;
+                                tmp64_1 <- (tmp64_1 + tmp64_2);
+                                tmp64_2 <- numbers_min;
+                                tmp64_1 <- (tmp64_1 + tmp64_2);
+                                tmp64_2 <- special_min;
+                                tmp64_1 <- (tmp64_1 + tmp64_2);
+                                if ((tmp64_1 \ule length)) {
+                                  tmp64_1 <- lowercase_max;
+                                  tmp64_2 <- uppercase_max;
+                                  tmp64_1 <- (tmp64_1 + tmp64_2);
+                                  tmp64_2 <- numbers_max;
+                                  tmp64_1 <- (tmp64_1 + tmp64_2);
+                                  tmp64_2 <- special_max;
+                                  tmp64_1 <- (tmp64_1 + tmp64_2);
+                                  if ((length \ule tmp64_1)) {
+                                    lowercase_set.[0] <- (W8.of_int 97);
+                                    lowercase_set.[1] <- (W8.of_int 98);
+                                    lowercase_set.[2] <- (W8.of_int 99);
+                                    lowercase_set.[3] <- (W8.of_int 100);
+                                    lowercase_set.[4] <- (W8.of_int 101);
+                                    lowercase_set.[5] <- (W8.of_int 102);
+                                    lowercase_set.[6] <- (W8.of_int 103);
+                                    lowercase_set.[7] <- (W8.of_int 104);
+                                    lowercase_set.[8] <- (W8.of_int 105);
+                                    lowercase_set.[9] <- (W8.of_int 106);
+                                    lowercase_set.[10] <- (W8.of_int 107);
+                                    lowercase_set.[11] <- (W8.of_int 108);
+                                    lowercase_set.[12] <- (W8.of_int 109);
+                                    lowercase_set.[13] <- (W8.of_int 110);
+                                    lowercase_set.[14] <- (W8.of_int 111);
+                                    lowercase_set.[15] <- (W8.of_int 112);
+                                    lowercase_set.[16] <- (W8.of_int 113);
+                                    lowercase_set.[17] <- (W8.of_int 114);
+                                    lowercase_set.[18] <- (W8.of_int 115);
+                                    lowercase_set.[19] <- (W8.of_int 116);
+                                    lowercase_set.[20] <- (W8.of_int 117);
+                                    lowercase_set.[21] <- (W8.of_int 118);
+                                    lowercase_set.[22] <- (W8.of_int 119);
+                                    lowercase_set.[23] <- (W8.of_int 120);
+                                    lowercase_set.[24] <- (W8.of_int 121);
+                                    lowercase_set.[25] <- (W8.of_int 122);
+                                    i <- (W64.of_int 26);
+                                    
+                                    while ((i \ult (W64.of_int 76))) {
+                                      lowercase_set.[(W64.to_uint i)] <-
+                                      (W8.of_int 0);
+                                      i <- (i + (W64.of_int 1));
+                                    }
+                                    uppercase_set.[0] <- (W8.of_int 65);
+                                    uppercase_set.[1] <- (W8.of_int 66);
+                                    uppercase_set.[2] <- (W8.of_int 67);
+                                    uppercase_set.[3] <- (W8.of_int 68);
+                                    uppercase_set.[4] <- (W8.of_int 69);
+                                    uppercase_set.[5] <- (W8.of_int 70);
+                                    uppercase_set.[6] <- (W8.of_int 71);
+                                    uppercase_set.[7] <- (W8.of_int 72);
+                                    uppercase_set.[8] <- (W8.of_int 73);
+                                    uppercase_set.[9] <- (W8.of_int 74);
+                                    uppercase_set.[10] <- (W8.of_int 75);
+                                    uppercase_set.[11] <- (W8.of_int 76);
+                                    uppercase_set.[12] <- (W8.of_int 77);
+                                    uppercase_set.[13] <- (W8.of_int 78);
+                                    uppercase_set.[14] <- (W8.of_int 79);
+                                    uppercase_set.[15] <- (W8.of_int 80);
+                                    uppercase_set.[16] <- (W8.of_int 81);
+                                    uppercase_set.[17] <- (W8.of_int 82);
+                                    uppercase_set.[18] <- (W8.of_int 83);
+                                    uppercase_set.[19] <- (W8.of_int 84);
+                                    uppercase_set.[20] <- (W8.of_int 85);
+                                    uppercase_set.[21] <- (W8.of_int 86);
+                                    uppercase_set.[22] <- (W8.of_int 87);
+                                    uppercase_set.[23] <- (W8.of_int 88);
+                                    uppercase_set.[24] <- (W8.of_int 89);
+                                    uppercase_set.[25] <- (W8.of_int 90);
+                                    i <- (W64.of_int 26);
+                                    
+                                    while ((i \ult (W64.of_int 76))) {
+                                      uppercase_set.[(W64.to_uint i)] <-
+                                      (W8.of_int 0);
+                                      i <- (i + (W64.of_int 1));
+                                    }
+                                    numbers_set.[0] <- (W8.of_int 48);
+                                    numbers_set.[1] <- (W8.of_int 49);
+                                    numbers_set.[2] <- (W8.of_int 50);
+                                    numbers_set.[3] <- (W8.of_int 51);
+                                    numbers_set.[4] <- (W8.of_int 52);
+                                    numbers_set.[5] <- (W8.of_int 53);
+                                    numbers_set.[6] <- (W8.of_int 54);
+                                    numbers_set.[7] <- (W8.of_int 55);
+                                    numbers_set.[8] <- (W8.of_int 56);
+                                    numbers_set.[9] <- (W8.of_int 57);
+                                    i <- (W64.of_int 10);
+                                    
+                                    while ((i \ult (W64.of_int 76))) {
+                                      numbers_set.[(W64.to_uint i)] <-
+                                      (W8.of_int 0);
+                                      i <- (i + (W64.of_int 1));
+                                    }
+                                    special_set.[0] <- (W8.of_int 33);
+                                    special_set.[1] <- (W8.of_int 63);
+                                    special_set.[2] <- (W8.of_int 35);
+                                    special_set.[3] <- (W8.of_int 36);
+                                    special_set.[4] <- (W8.of_int 37);
+                                    special_set.[5] <- (W8.of_int 38);
+                                    special_set.[6] <- (W8.of_int 43);
+                                    special_set.[7] <- (W8.of_int 45);
+                                    special_set.[8] <- (W8.of_int 42);
+                                    special_set.[9] <- (W8.of_int 95);
+                                    special_set.[10] <- (W8.of_int 64);
+                                    special_set.[11] <- (W8.of_int 58);
+                                    special_set.[12] <- (W8.of_int 59);
+                                    special_set.[13] <- (W8.of_int 61);
+                                    i <- (W64.of_int 14);
+                                    
+                                    while ((i \ult (W64.of_int 76))) {
+                                      special_set.[(W64.to_uint i)] <-
+                                      (W8.of_int 0);
+                                      i <- (i + (W64.of_int 1));
+                                    }
+                                    i <- (W64.of_int 0);
+                                    
+                                    while ((i \ult (W64.of_int 76))) {
+                                      union_set.[(W64.to_uint i)] <-
+                                      (W8.of_int 0);
+                                      i <- (i + (W64.of_int 1));
+                                    }
+                                    i_filled <- (W64.of_int 0);
+                                    if (((W64.of_int 0) \ult lowercase_max)) {
+                                      i <- (W64.of_int 0);
+                                      
+                                      while ((i \ult lowercase_min)) {
+                                        lowercase_max <-
+                                        (lowercase_max - (W64.of_int 1));
+                                        tmp8 <@ random_char_generator ((W64.of_int 26),
+                                        lowercase_set);
+                                        Glob.mem <-
+                                        storeW8 Glob.mem (W64.to_uint (output_addr + i_filled)) tmp8;
+                                        i <- (i + (W64.of_int 1));
+                                        i_filled <-
+                                        (i_filled + (W64.of_int 1));
+                                      }
+                                    } else {
+                                      
+                                    }
+                                    if (((W64.of_int 0) \ult uppercase_max)) {
+                                      i <- (W64.of_int 0);
+                                      
+                                      while ((i \ult uppercase_min)) {
+                                        uppercase_max <-
+                                        (uppercase_max - (W64.of_int 1));
+                                        tmp8 <@ random_char_generator ((W64.of_int 26),
+                                        uppercase_set);
+                                        Glob.mem <-
+                                        storeW8 Glob.mem (W64.to_uint (output_addr + i_filled)) tmp8;
+                                        i <- (i + (W64.of_int 1));
+                                        i_filled <-
+                                        (i_filled + (W64.of_int 1));
+                                      }
+                                    } else {
+                                      
+                                    }
+                                    if (((W64.of_int 0) \ult numbers_max)) {
+                                      i <- (W64.of_int 0);
+                                      
+                                      while ((i \ult numbers_min)) {
+                                        numbers_max <-
+                                        (numbers_max - (W64.of_int 1));
+                                        tmp8 <@ random_char_generator ((W64.of_int 10),
+                                        numbers_set);
+                                        Glob.mem <-
+                                        storeW8 Glob.mem (W64.to_uint (output_addr + i_filled)) tmp8;
+                                        i <- (i + (W64.of_int 1));
+                                        i_filled <-
+                                        (i_filled + (W64.of_int 1));
+                                      }
+                                    } else {
+                                      
+                                    }
+                                    if (((W64.of_int 0) \ult special_max)) {
+                                      i <- (W64.of_int 0);
+                                      
+                                      while ((i \ult special_min)) {
+                                        special_max <-
+                                        (special_max - (W64.of_int 1));
+                                        tmp8 <@ random_char_generator ((W64.of_int 14),
+                                        special_set);
+                                        Glob.mem <-
+                                        storeW8 Glob.mem (W64.to_uint (output_addr + i_filled)) tmp8;
+                                        i <- (i + (W64.of_int 1));
+                                        i_filled <-
+                                        (i_filled + (W64.of_int 1));
+                                      }
+                                    } else {
+                                      
+                                    }
                                     (tmp64_1,
                                     union_set) <@ define_union_set (lowercase_max,
                                     uppercase_max, numbers_max, special_max,
                                     lowercase_set, uppercase_set,
                                     numbers_set, special_set, union_set);
-                                  } else {
+                                    tmp64_2 <- length;
                                     
+                                    while ((i_filled \ult tmp64_2)) {
+                                      tmp8 <@ random_char_generator (tmp64_1,
+                                      union_set);
+                                      if (((W8.of_int 97) \ule tmp8)) {
+                                        if ((tmp8 \ule (W8.of_int 122))) {
+                                          lowercase_max <-
+                                          (lowercase_max - (W64.of_int 1));
+                                          if ((lowercase_max = (W64.of_int 0))) {
+                                            (tmp64_1,
+                                            union_set) <@ define_union_set (lowercase_max,
+                                            uppercase_max, numbers_max,
+                                            special_max, lowercase_set,
+                                            uppercase_set, numbers_set,
+                                            special_set, union_set);
+                                          } else {
+                                            
+                                          }
+                                        } else {
+                                          
+                                        }
+                                      } else {
+                                        if (((W8.of_int 65) \ule tmp8)) {
+                                          if ((tmp8 \ule (W8.of_int 90))) {
+                                            uppercase_max <-
+                                            (uppercase_max - (W64.of_int 1));
+                                            if ((uppercase_max = (W64.of_int 0))) {
+                                              (tmp64_1,
+                                              union_set) <@ define_union_set (lowercase_max,
+                                              uppercase_max, numbers_max,
+                                              special_max, lowercase_set,
+                                              uppercase_set, numbers_set,
+                                              special_set, union_set);
+                                            } else {
+                                              
+                                            }
+                                          } else {
+                                            
+                                          }
+                                        } else {
+                                          if (((W8.of_int 48) \ule tmp8)) {
+                                            if ((tmp8 \ule (W8.of_int 57))) {
+                                              numbers_max <-
+                                              (numbers_max - (W64.of_int 1));
+                                              if ((numbers_max = (W64.of_int 0))) {
+                                                (tmp64_1,
+                                                union_set) <@ define_union_set (lowercase_max,
+                                                uppercase_max, numbers_max,
+                                                special_max, lowercase_set,
+                                                uppercase_set, numbers_set,
+                                                special_set, union_set);
+                                              } else {
+                                                
+                                              }
+                                            } else {
+                                              
+                                            }
+                                          } else {
+                                            special_max <-
+                                            (special_max - (W64.of_int 1));
+                                            if ((special_max = (W64.of_int 0))) {
+                                              (tmp64_1,
+                                              union_set) <@ define_union_set (lowercase_max,
+                                              uppercase_max, numbers_max,
+                                              special_max, lowercase_set,
+                                              uppercase_set, numbers_set,
+                                              special_set, union_set);
+                                            } else {
+                                              
+                                            }
+                                          }
+                                        }
+                                      }
+                                      Glob.mem <-
+                                      storeW8 Glob.mem (W64.to_uint (output_addr + i_filled)) tmp8;
+                                      i_filled <-
+                                      (i_filled + (W64.of_int 1));
+                                    }
+                                    tmp64_1 <- length;
+                                    permutation (output_addr, tmp64_1);
+                                    Glob.mem <-
+                                    storeW64 Glob.mem (W64.to_uint (output_addr + tmp64_1)) (W64.of_int 0);
+                                    output <- (W64.of_int 1);
+                                  } else {
+                                    output <- (W64.of_int (- 16));
                                   }
                                 } else {
-                                  
+                                  output <- (W64.of_int (- 15));
                                 }
                               } else {
-                                if (((W8.of_int 65) \ule tmp8)) {
-                                  if ((tmp8 \ule (W8.of_int 90))) {
-                                    uppercase_max <-
-                                    (uppercase_max - (W64.of_int 1));
-                                    if ((uppercase_max = (W64.of_int 0))) {
-                                      (tmp64_1,
-                                      union_set) <@ define_union_set (lowercase_max,
-                                      uppercase_max, numbers_max,
-                                      special_max, lowercase_set,
-                                      uppercase_set, numbers_set,
-                                      special_set, union_set);
-                                    } else {
-                                      
-                                    }
-                                  } else {
-                                    
-                                  }
-                                } else {
-                                  if (((W8.of_int 48) \ule tmp8)) {
-                                    if ((tmp8 \ule (W8.of_int 57))) {
-                                      numbers_max <-
-                                      (numbers_max - (W64.of_int 1));
-                                      if ((numbers_max = (W64.of_int 0))) {
-                                        (tmp64_1,
-                                        union_set) <@ define_union_set (lowercase_max,
-                                        uppercase_max, numbers_max,
-                                        special_max, lowercase_set,
-                                        uppercase_set, numbers_set,
-                                        special_set, union_set);
-                                      } else {
-                                        
-                                      }
-                                    } else {
-                                      
-                                    }
-                                  } else {
-                                    special_max <-
-                                    (special_max - (W64.of_int 1));
-                                    if ((special_max = (W64.of_int 0))) {
-                                      (tmp64_1,
-                                      union_set) <@ define_union_set (lowercase_max,
-                                      uppercase_max, numbers_max,
-                                      special_max, lowercase_set,
-                                      uppercase_set, numbers_set,
-                                      special_set, union_set);
-                                    } else {
-                                      
-                                    }
-                                  }
-                                }
+                                output <- (W64.of_int (- 14));
                               }
-                              Glob.mem <-
-                              storeW8 Glob.mem (W64.to_uint (output_addr + i_filled)) tmp8;
-                              i_filled <- (i_filled + (W64.of_int 1));
+                            } else {
+                              output <- (W64.of_int (- 13));
                             }
-                            tmp64_1 <- length;
-                            permutation (output_addr, tmp64_1);
-                            Glob.mem <-
-                            storeW64 Glob.mem (W64.to_uint (output_addr + tmp64_1)) (W64.of_int 0);
-                            output <- (W64.of_int 1);
                           } else {
                             output <- (W64.of_int (- 12));
                           }
